lib/Benchmarks/EthernetProof.v
@@ -4,6 +4,7 @@ Require Import Leapfrog.Benchmarks.Ethernet.
 Declare ML Module "mirrorsolve".
 SetSMTSolver "cvc4".
 
+
 Lemma ethernet_equiv:
   lang_equiv_state
     (P4A.interp Reference.aut)
@@ -11,5 +12,14 @@ Lemma ethernet_equiv:
     Reference.SPref
     Combined.Parse.
 Proof.
-  solve_lang_equiv_state_axiom Reference.state_eqdec Combined.state_eqdec false.
-Time Qed.
+  eapply lang_equiv_to_pre_bisim;
+  time "init prebisim" (intros;
+  unfold mk_init;
+  erewrite Reachability.reachable_states_wit_conv; [
+    | repeat econstructor
+    | unfold Reachability.reachable_states_wit;
+      solve_fp_wit
+  ]; simpl).
+Admitted.
+  (* solve_lang_equiv_state_axiom Reference.state_eqdec Combined.state_eqdec false.
+Time Qed. *)
